### Proposición

Sea $f: V \rightarrow V'$ lineal, entonces:
1. $f(0_v) = 0_{v'}$.
2. $\forall v \in V, \forall \lambda \in K, f(\lambda v) = \lambda f(v)$.

---
### Demostración

1. $f(0) = f(1 · 0 + 1 · 0)$. Como $f$ es lineal, $f(1·0 + 1·0) = 1 · f(0) + 1 · f(0) = f(0) + f(0)$. Sumando la inversa de $f(0)$ a ambos lados: $f(0) + (-f(0)) = f(0) + f(0) + (-f(0)) \implies f(0) = 0$.
2. $f(\lambda v) = f(\lambda v + 1 · 0)$. Como $f$ es lineal, $f(\lambda v + 1·0) = \lambda f(v) + 1 · f(0) = \lambda f(v)$ (1).

---
### Referencias

[[Aplicación lineal]]

24-10-23. Álgebra lineal.