### Proposición

Sea $(A,+,·)$ anillo, $e$ neutro de $+$ y $-a$ el simétrico de $a$ para $+$, entonces:
- $a · e = e = e · a, \forall a \in A$.
- $(-a) · b = -(a·b) = a · (-b)$.

---
### Demostración

Veamos que $a · e = e$, $a · e + a · e = a(e+e) = a · e = a·e + e \implies -(a · e) + a · e + a · e = -(a·e) + a·e + e \implies a · e = e$.

Veamos que $(-a) · b = -(a·b) = a · (-b)$. Tenemos que ver que $(-a) · b + a · b = ((-a)+a) ·b = -e · b  = e \implies a · b + (-a) ·b = e$, dado que $+$ es conmutativo.

---
### Referencias
[[Anillo]]
[[Estructuras algebraicas elementales]]

19-10-23. Matemática Básica.