### Contenido principal

Se denota como $s^2$, y se mide en en $cm^2$:
$$
\begin{equation}
s^2 = \frac{1}{n-1} \sum^n_{i=1}(x-\overline{x})^2
\end{equation}
$$

Vamos a desarrollar la varianza:
$s^2 = \frac{1}{n-1} (\sum^n_{i=1} (x^2_i - 2\overline{x}x_i + \overline{x}^2))$
$s^2 = \frac{1}{n-1} (\sum^n_{i=1}x^2_i - 2\overline{x}\sum_{i=1}^n x_i + \overline{x}^2 \sum^n_{i=1}1)$
$s^2 = \frac{1}{n-1} (\sum^n_{i=1}x^2_i - 2\overline{x}^2 n + \overline{x}^2 n)$ porque $n\overline{x} = \sum_{i=1}^n x_i$ y $\sum^n_{i=1} 1 = n$.
$s^2 = \frac{1}{n-1} \sum^n_{i=1} (x^2_i - \overline{x}^2 n)$.


--- 
### Referencias
[[Medidas de dispersiÃ³n]]