### Proposición

Sean $\sum^{+\infty}_{n=1} a_n$ y $\sum_{n=1}^{+\infty} b_n$ convergentes a $S_1$ y $S_2$ respectivamente, entonces $\sum_{n=1}^{+\infty} (\alpha a_n + \beta b_n)$ converge a $\alpha S_1$ y $\beta S_2$. Escribimos $\sum^{+\infty}_{n=1} (\alpha a_n + \beta b_n) = \alpha \sum^{+\infty}_{n=1}a_n + \beta \sum_{n=1}^{+\infty} b_n$.

---
### Demostración

$\sum_{n=1}^{+\infty} (\alpha a_n + \beta b_n) = lim_{N \to +\infty} \sum_{n=1}^{N} (\alpha a_n + \beta b_n) = \alpha lim_{N \to +\infty} \sum_{n=1}^{N} a_n + \beta lim_{N \to +\infty} \sum_{n=1}^{N} b_n =$ $\alpha \sum_{n=1}^{+\infty} a_n + \beta \sum_{n=1}^{+\infty} b_n$
Similar a la primera de las [[Propiedades para el cálculo de límites]]

---
### Referencias
[[Serie numérica]]