
---
mathLink:
---
### Contenido Principal

**Fecha:** 2024-04-29, 18:58

```ad-lemma
Sea $f: [a,b] \to \mathbb R$ acotada, $I \subset [a,b]$. Sean:
$$\begin{array}{c c}
M_I = \sup \{f(x): x \in I \} & m_I = \inf \{f(x) : x \in I \} \\
M_I' = \sup \{|f(x)| : x \in I \} & m_I' = \inf \{|f(x)| : x \in I \}.
\end{array}$$
Entonces,
1. $M_I - m_I = \sup \{f(x) - f(y) : x,y \in I \} = \sup \{|f(x) - f(y)|: x,y \in I \}.$
2. $M_I' - m_I' \le M_I - m_I.$
```


```ad-proof

```



**Tema:** [[Integración de funciones de una variable real]]
**Corolarios:**

---
### Anki

START
Respuesta anidada
Sea $f: [a,b] \to \mathbb R$ acotada, $I \subset [a,b]$. Sean:
$$\begin{array}{c c}
M_I = \sup \{f(x): x \in I \} & m_I = \inf \{f(x) : x \in I \} \\
M_I' = \sup \{|f(x)| : x \in I \} & m_I' = \inf \{|f(x)| : x \in I \}.
\end{array}$$
Entonces,
{{c1::1. $M_I - m_I = \sup \{f(x) - f(y) : x,y \in I \} = \sup \{|f(x) - f(y)|: x,y \in I \}.$}}
{{c2::2. $M_I' - m_I' \le M_I - m_I.$}}
Tags: proposición/teorema análisisI
<!--ID: 1714669443757-->
END
